\documentclass[12pt]{article}
\usepackage[margin=1in]{geometry}
\usepackage{amsthm, hhline, enumitem}
\usepackage{stmaryrd, mathtools}
\usepackage{amsmath, amssymb, graphicx}
\usepackage{mathtools}
\usepackage{bbm}
\newtheorem{theorem}{Theorem}
\newtheorem{lemma}{Lemma}
\newtheorem{cor}{Corollary}
\newtheorem*{lemma*}{Lemma}
\newtheorem*{theorem*}{Theorem}
{ \theoremstyle{remark}
	\newtheorem{remark}[theorem]{Remark}}
{ \theoremstyle{definition}
	\newtheorem{definition}[theorem]{Definition}}
\DeclareMathOperator{\ex}{\mathbb{E}}
\DeclareMathOperator{\pr}{\mathbb{P}}
\DeclareMathOperator{\indic}{\mathbbm{1}}
\DeclareMathOperator{\cov}{cov}
\DeclareMathOperator{\var}{var}
\DeclareMathOperator{\sgn}{sgn}
\DeclarePairedDelimiter\ceil{\lceil}{\rceil}
\DeclarePairedDelimiter\floor{\lfloor}{\rfloor}
\DeclarePairedDelimiter\abs{\lvert}{\rvert}
\begin{document}
	\begin{flushright}
		Summer 2020
	\end{flushright}
	
	\begin{center}
		\LARGE\textbf{REU Practice Problems}
	\end{center}


\section{Topology and measurability}

\subsection*{Problem 19}
Fix $p \in (0,1)$, $k \in \mathbb{N}$. Suppose that $\vec{x}^T = (x^T_1, \dots, x^T_k)$ and $\vec{y}^T = (y^T_1, \dots, y^T_k)$ is a sequence of $k$-dimensional vectors with integer entries such that $T\geq y_i^T -x_i^T \geq 0$ for $i = 1, \dots k$. Find constants $A,B,C >0$ depending on $p$ such that the following holds. For any $M_1, M_2 > 0$ there exists a $T_0 \in \mathbb{N}$ depending on $p,k,M_1,M_2, M$ such that if $T \geq T_0$, $x_k^T \geq - M_1 \sqrt{T}$ and $y_k^T \geq pT - M_2 \sqrt{T}$ then 
$$\mathbb{P}_{avoid, Ber}^{0,T, \vec{x}^T, \vec{y}^T} \left( L_k(T/2) - (pT/2) \geq M \sqrt{T} \right) \geq A \cdot \exp \left( - Bk (M_1 + M_2 + M + C)^2 \right).$$

\begin{proof}
Define events
$$ A:=\left\{ L_k\left(\frac{T}{2}\right)-\frac{pT}{2} \geq M\sqrt{T}) \right\}$$
$$ B:=\left\{ L_1(s)>\dots>L_k(s) , s \in [0,T]\right\}$$
We aim to find a lower bound for $\mathbb{P}_{avoid, Ber}^{0,T, \vec{x}^T, \vec{y}^T} (A)
= \mathbb{P}_{Ber}^{0,T, \vec{x}^T, \vec{y}^T}  (A|B)$.
It follows from Lemma 3.1 that if we lower the endpoints of each curve, the probability of the event A will decrease. 
In particular, define $\vec{x}\,'^T = (\vec{x_1}'^T,\dots,\vec{x_k}'^T)$ and $\vec{y}\,'^T = (\vec{y_1}'^T,\dots,\vec{y_k}'^T)$ by
\begin{align*}
x_i'^T &= \lfloor x_i^T - C(i-1)\sqrt{T} \rfloor  \text{ for } i=1,\dots,k-1\text{, and } x_k'^T= \lfloor -M_1\sqrt{T} - C(k-1)\sqrt{T} \rfloor\\
y_i'^T &= \lfloor y_i'^T-C(i-1)\sqrt{T} \rfloor \text{ for } i=1,\dots,k-1\text{, and }y_k'^T= \lfloor pT-M_2\sqrt{T} - C(k-1)\sqrt{T} \rfloor
\end{align*}
In which $C$ is a constant which we will specify. Note that $x_k'^T<x_i'^T < x_i^T$ for each $i$, and that $x_i'^T-x_{i+1}'^T>C\sqrt{T}$. The same holds for $y_i'^T$. For simplicity, we denote $ \mathbb{P}_{Ber}^{0,T, \vec{x}\,'^T, \vec{y}\,'^T}$ by $\mathbb{P'}$. Lemma 3.1 implies

\begin{align*}
\mathbb{P}_{avoid, Ber}^{0,T, \vec{x}^T, \vec{y}^T}(A) 
=& \mathbb{P}_{Ber}^{0,T, \vec{x}^T, \vec{y}^T}(A|B) \\
\geq& \mathbb{P}_{Ber}^{0,T, \vec{x}\,'^T, \vec{y}\,'^T}(A|B) \\
=& \mathbb{P'}(A|B)\\
=& 1 -  \mathbb{P'}(A^c|B)\\
=& 1 -  \frac{\mathbb{P'}(A^c\cap B)}{\mathbb{P'}(B)} \\
\geq& 1 -  \frac{\mathbb{P'}(A^c)}{\mathbb{P'}(B)} \\
=&  1 -  \frac{1-\mathbb{P'}(A)}{\mathbb{P'}(B)}
\end{align*}
We proceed to find lower bounds for $\mathbb{P'}(A)$, and for $\mathbb{P'}(B)$.

\noindent\textbf{Step 1:} 
 We know from the same reasoning as in Lemma 3.9 that
\begin{align*}
\mathbb{P'}(A)
= & \mathbb{P}_{Ber}^{0,T, \vec{x}\,'^T, \vec{y}\,'^T} \left(L_k\left(\frac{T}{2}\right)-\frac{pT}{2} \geq M\sqrt{T}) \right) \\
\geq & \mathbb{P}_{Ber}^{0,T, x_k'^T, y_k'^T}\left(l\left(\frac{T}{2}\right)-\frac{pT}{2} \geq M\sqrt{T}) \right) \\
= & \mathbb{P}\left(l^{(T,z)} \left(\frac{T}{2}\right)-\frac{pT}{2} \geq M\sqrt{T}) \right)
\end{align*}
where $z:= y_k'^T-x_k'^T = \lfloor M_1\sqrt{T}+pT-M_2\sqrt{T} \rfloor$, and $\mathbb{P}$, $l^{(T,z)}$ are as defined in Theorem 3.3.
With Brownian bridge $B^\sigma$ as in Theorem 3.3. We rewrite the expression as

\begin{align*}
\mathbb{P} \left( \left[ l^{(T,z)} \left(\frac{T}{2}\right)
-\sqrt{T}B^\sigma_{1/2}-\frac{z}{2} \right] + \sqrt{T}B^\sigma  
\geq -\frac{M_1\sqrt{T}-M_2\sqrt{T}}{2} + M\sqrt{T}) \right)
\end{align*}
Cleaning up, we have
$$-\frac{M_1\sqrt{T}-M_2\sqrt{T}}{2} + M\sqrt{T} = (M+\frac{M_2-M_1}{2})\sqrt{T} $$
The probability $\mathbb{P'}(A)$ is bounded below by
\begin{align*}
& \mathbb{P} \left( \left[ l^{(T,z)} \left(\frac{T}{2}\right)
-\sqrt{T}B^\sigma_{1/2}-\frac{z}{2} \right] + \sqrt{T}B^\sigma  
\geq (M+\frac{M_2-M_1}{2})\sqrt{T} \right) \\
\geq& \mathbb{P} \left( B^\sigma_{1/2} \geq M_1+M_2 \right)
\end{align*}

\noindent\textbf{Step 2:} 
Now it remains to lower bound $\mathbb{P'}(B)$. We write
\begin{align*}
\mathbb{P'}(B) &= \mathbb{P}_{Ber}^{0,T, \vec{x}\,'^T, \vec{y}\,'^T} \left( L_1(s)>\dots>L_k(s), s\in[0,T]\right) \\
&\geq  \mathbb{P}_{Ber}^{0,T, \vec{x}\,'^T, \vec{y}\,'^T} \left( \sup_{s\in[0,T]}
 | L_i(s)-x_i'-\frac{s}{T}(y_i-x_i) | \leq \frac{C\sqrt{T}}{2}, 1\leq i \leq k \right) \\
 &=  \left[ 1 - \mathbb{P}_{Ber}^{0,T, \vec{x}\,'^T, \vec{y}\,'^T} \left( \sup_{s\in[0,T]}
 | L_i(s)-x_i'-\frac{s}{T}(y_i-x_i) | > \frac{C\sqrt{T}}{2}, 1\leq i \leq k \right) \right]^k
\end{align*}
We know that
\begin{align*}
&\mathbb{P}_{Ber}^{0,T, \vec{x}\,'^T, \vec{y}\,'^T} \left( \sup_{s\in[0,T]}
 | L_i(s)-x_i'-\frac{s}{T}(y_i'-x_i') | > \frac{C\sqrt{T}}{2}, 1\leq i \leq k \right) \\
 \leq& \mathbb{P}\left( \sup_{s\in[0,T]} |\sqrt{T} B^\sigma _\frac{s}{T}| > \frac{C\sqrt{T}}{4} \right)
 + \mathbb{P} \left( \Delta(T, y_i'-x_i')>\frac{C\sqrt{T}}{4} \right) \\
 =& 2\exp\left(-\frac{2}{\sigma^2}(\frac{C}{4})^2\right) - O(\exp(-\sqrt{T})) 
 \end{align*}
Since
$$\mathbb{P'}(B) = \left( 1 - 2\exp\left(-\frac{2}{\sigma^2}(\frac{C}{4})^2\right) + O(\exp(-\sqrt{T}))  \right)^k$$
we can find some $T>T_0$ such that $\mathbb{P'}(B)  > \frac{m}{n} $ for given integers $m,n$. We could pick $m,n$ such that $m< (1-\frac{\mathbb{P'}(A)}{2-\mathbb{P'}(A)})n$. We will have
\begin{align*}
\mathbb{P}_{avoid, Ber}^{0,T, \vec{x}^T, \vec{y}^T}(A) 
\geq&  1 -  \frac{1-\mathbb{P'}(A)}{\mathbb{P'}(B)} \\
=& 1+\frac{n}{m} (\mathbb{P'}(A)-1) \\
\geq & \frac{1}{2}\mathbb{P'}(A)
\end{align*}
whose boundedness was proven in Step 1.
\end{proof}


\end{document}
