%-------------------------------------------------------------------------------------------------------------------------------------------------------------------------------------------------
% Section 4
%
%-------------------------------------------------------------------------------------------------------------------------------------------------------------------------------------------------
\section{Proof of Theorem \ref{PropTightGood} }\label{Section4}


The goal of this section is to prove Theorem \ref{PropTightGood} and for the remainder of this section we assume that $k \in \mathbb{N}$ with $k \geq 2$, $p \in (0,1)$, $\alpha, \lambda > 0$ are all fixed and 
\begin{equation*}
\big\{\mathfrak{L}^N = (L^N_1,L^N_2, \dots, L^N_k)\big\}_{N=1}^{\infty},
\end{equation*}
is an $(\alpha,p,\lambda)$-good sequence of $\llbracket 1, k\rrbracket$-indexed Bernoulli line ensembles as in Definition \ref{Def1} that are all defined on a probability space with measure $\mathbb{P}$. The proof of Theorem \ref{PropTightGood} depends on three results -- Proposition \ref{PropMain} and Lemmas \ref{PropSup} and \ref{PropSup2}. In these three statements we establish various properties of the sequence of line ensembles $\mathfrak{L}^N$ and the constants in those statements depend implicitly on $\alpha$, $p$, $\lambda$, $k$, and the functions $\phi, \psi$ from Definition \ref{Def1}, which are fixed throughout. We will not list this dependence explicitly. The proof of Proposition \ref{PropMain} is given in Section \ref{Section4.1} while the proofs of Lemmas \ref{PropSup} and \ref{PropSup2} are in Section \ref{Section5}. Theorem \ref{PropTightGood} is proved in Section \ref{Section4.2}.
%-------------------------------------------------------------------------------------------------------------------------------------------------------------------------------------------------
% Section 4.1
%
%-------------------------------------------------------------------------------------------------------------------------------------------------------------------------------------------------
\subsection{Bounds on the acceptance probability}\label{Section4.1}
The main result in this section is presented as Proposition \ref{PropMain} below. In order to formulate it and some of the lemmas below it will be convenient to adopt the following notation for any $r > 0$ and $m \in \mathbb{N}$
\begin{equation}\label{eqsts}
t_m =\lfloor (r+m) N^{\alpha} \rfloor.
\end{equation}
\begin{proposition}\label{PropMain} Let $\mathbb{P}$ be the measure from the beginning of this section. For any $\epsilon > 0$, $r > 0$ there exist $\delta = \delta(\epsilon, r) > 0$ and $N_1 = N_1(\epsilon, r)$ such that for all $N \geq N_1$
	we have 
	$$\mathbb{P}\Big(Z\big( -t_1, t_1, \vec{x}, \vec{y} , \infty,  L^N_{k}\llbracket -t_1, t_1\rrbracket\big) < \delta\Big) < \epsilon,$$
	where $\vec{x} = (L_1^N(-t_1), \dots, L_{k-1}^N(-t_1))$, $\vec{y} = (L_1^N(t_1), \dots, L^N_{k-1}(t_1))$,  $ L^N_{k}\llbracket -t_1, t_1\rrbracket$ is the restriction of $L^N_k$ to the set $\llbracket -t_1, t_1\rrbracket$, and $Z$ is the acceptance probability of Definition \ref{DefAP}. 
\end{proposition}

The general strategy we use to prove Proposition \ref{PropMain} is inspired by the proof of \cite[Proposition 6.5]{CorHamK}. We begin by stating three key lemmas that will be required. The proofs of Lemmas \ref{PropSup} and \ref{PropSup2} are postponed to Section \ref{Section5} and Lemma \ref{LemmaAP1} is proved in Section \ref{Section6}.


\begin{lemma}\label{PropSup}  Let $\mathbb{P}$ be the measure from the beginning of this section. For any $\epsilon > 0$, $r > 0$ there exist $R_1=R_1(\epsilon,r) > 0$ and $N_2= N_2(\epsilon,r)$ such that for $N \geq N_2$ 
	$$\mathbb{P} \left( \sup_{s \in [ -t_3, t_3] }\big[ L^N_1(s) - p s \big] \geq  R_1N^{\alpha/2} \right) < \epsilon.$$
\end{lemma}

\begin{lemma}\label{PropSup2}  Let $\mathbb{P}$ be the measure from the beginning of this section.  For any $\epsilon > 0$, $r > 0$ there exist $R_2=R_2( \epsilon,r) > 0$ and $N_3=N_3(\epsilon,r)$ such that for $N \geq N_3$
	$$\mathbb{P}\left( \inf_{s \in [ -t_3, t_3 ]}\big[L^N_{k-1}(s) - p s \big] \leq - R_2N^{\alpha/2} \right) < \epsilon.$$
\end{lemma}

\begin{lemma}\label{LemmaAP1} Fix $k \in \mathbb{N}$, $k \geq 2$, $p \in (0,1)$, $r, \alpha, M_1, M_2 > 0$ . Suppose that $\ell_{bot}: \llbracket -t_3, t_3 \rrbracket \rightarrow \mathbb{R} \cup \{ - \infty \}$, and $\vec{x}, \vec{y} \in \mathfrak{W}_{k-1}$ are such that $|\Omega_{avoid}(-t_3, t_3, \vec{x}, \vec{y}, \infty, \ell_{bot})| \geq 1$. Suppose further that
	\begin{enumerate}
		\item $\sup_{s \in [- t_3,t_3]}\big[\ell_{bot}(s)  - ps \big]  \leq M_2 (2t_3)^{1/2}$,
		\item  $-pt_3 + M_1 (2t_3)^{1/2} \geq  x_1 \geq  x_{k-1} \geq \max\left(\ell_{bot}(-t_3), -pt_3- M_1 (2t_3)^{1/2}\right),$
		\item $pt_3 + M_1 (2t_3)^{1/2} \geq y_1 \geq y_{k-1} \geq  \max \left( \ell_{bot}(t_3),  p t_3- M_1(2t_3)^{1/2} \right).$
	\end{enumerate}
	Then there exist constants $g,h$ and $N_4 \in \mathbb{N}$ all depending on $ M_1, M_2, p , k, r, \alpha$   such that for any $\tilde{\epsilon}  > 0$ and $N \geq N_4$ we have
	\begin{equation}\label{eqn60}
	\mathbb{P}^{-t_3, t_3, \vec{x},\vec{y}, \infty, \ell_{bot} }_{avoid, Ber} \Big( Z\big(  -t_1, t_1, \mathfrak{Q}(-t_1) ,\mathfrak{Q}(t_1), \infty,  \ell_{bot}\llbracket -t_1, t_1\rrbracket\big) \leq  gh \tilde{\epsilon}   \Big)  \leq \tilde{\epsilon},
	\end{equation}
	where $Z$ is the acceptance probability of Definition \ref{DefAP}, $\ell_{bot}\llbracket -t_1, t_1\rrbracket$ is the vector, whose coordinates match those of $\ell_{bot}$ on $\llbracket -t_1, t_1\rrbracket$ and $\mathfrak{Q}(a) = (Q_1(a), \dots, Q_{k-1}(a))$ is the value of the line ensemble $\mathfrak{Q} = (Q_1, \dots, Q_{k-1})$ whose law is $\mathbb{P}^{-t_3, t_3, \vec{x},\vec{y}, \infty, \ell_{bot} }_{avoid, Ber}$ at location $a$.
\end{lemma}


\begin{proof}[Proof of Proposition \ref{PropMain}] Let $\epsilon > 0$ be given. Define the event
	\begin{equation*}
	\begin{split}
	E_N = &\left\{    L_{k-1}^N(  \pm t_3) \mp pt_3 \geq  - M_1 (2t_3)^{1/2}\right\} \cap \left\{    L_{1}^N(  \pm t_3) \mp pt_3 \leq   M_1 (2t_3)^{1/2}\right\} \cap \\
	& \left\{ \sup_{s \in [ -t_3, t_3]} [{L}^N_{k}(s) - p s ]\leq M_2  (2t_3)^{1/2} \right\}.
	\end{split}
	\end{equation*}
	In view of  Lemmas \ref{PropSup} and \ref{PropSup2} and the fact that $\mathbb{P}$-almost surely $L_1^N(s) \geq L_k^N(s)$ for all $s \in [ -t_3, t_3]$ we can find sufficiently large $M_1, M_2$ and $N_2$ such that for $N \geq N_2$ we have 
	\begin{equation}\label{UBEC}
	\mathbb{P}(E_N^c) <  \epsilon / 2.
	\end{equation}
	
	
	Let $g,h, N_4$ be as in Lemma \ref{LemmaAP1} for the values $M_1, M_2$ as above, the values $\alpha, p, k$ from the beginning of the section and $r$ as in the statement of the proposition. For $\delta = (\epsilon/2) \cdot g h$ we denote
	$$V = \Big\{Z\big( -t_1,t_1, \vec{x}, \vec{y} , \infty,  L^N_{k}\llbracket -t_1, t_1\rrbracket\big)< \delta\Big\}$$
	and make the following deduction for $N \geq N_4$
	\begin{equation}\label{boundoneEN}
	\begin{split}
	&\mathbb{P}\big( V \cap E_N \big) =\mathbb{E} \bigg[    \mathbb{E}\Big[{\bf 1}_{E_N} \cdot {\bf 1}_{V} \Big{|} \sigma \big( \mathfrak{L}^N(-t_3),  \mathfrak{L}^N(t_3),L^N_k\llbracket -t_3, t_3\rrbracket   \big)\Big] \bigg] = \\
	&\mathbb{E} \bigg[ {\bf 1}_{E_N} \cdot   \mathbb{E}\Big[ {\bf 1} \{ Z\big( -t_1,t_1, \vec{x}, \vec{y} , \infty,  L^N_{k}\llbracket -t_1, t_1\rrbracket \big) < \delta\}   \Big{|} \sigma \big( \mathfrak{L}^N(-t_3),  \mathfrak{L}^N(t_3),L^N_k\llbracket -t_3, t_3\rrbracket   \big) \Big] \bigg]  = \\
	&\mathbb{E} \left[ {\bf 1}_{E_N} \cdot  \mathbb{E}_{avoid}\left[ {\bf 1} \{ Z\big( -t_1, t_1, \mathfrak{L}(-t_1),\mathfrak{L}(t_1), \infty, {L}^N_k\llbracket -t_1, t_1\rrbracket \big) < \delta\} \right] \right] \leq  \mathbb{E} \left[ {\bf 1}_{E_N} \cdot  \epsilon/2 \right] \leq \epsilon/2.
	\end{split}
	\end{equation}
	In (\ref{boundoneEN}) we have written $\mathbb{E}_{avoid}$ in place of $\mathbb{E}^{-t_3, t_3, \mathfrak{L}^N(-t_3), \mathfrak{L}^N(t_3), \infty, L^N_k\llbracket -t_3, t_3\rrbracket }_{avoid, Ber}$ to ease the notation; in addition, we have that $\mathfrak{L}^N(a) = (L_1^N(a), \dots, L_{k-1}^N(a))$ and $\mathfrak{L}$ on the last line is distributed according to $\mathbb{P}^{-t_3, t_3, \mathfrak{L}^N(-t_3), \mathfrak{L}^N(t_3), \infty, L^N_k\llbracket -t_3, t_3\rrbracket }_{avoid, Ber}$. We elaborate on (\ref{boundoneEN}) in the paragraph below.
	
	The first equality in (\ref{boundoneEN}) follows from the tower property for conditional expectations. The second equality uses the definition of $V$ and the fact that ${\bf 1}_{E_N} $ is $\sigma \big( \mathfrak{L}^N(-t_3),  \mathfrak{L}^N(t_3),L^N_k\llbracket -t_3, t_3\rrbracket   \big)$-measurable and can thus be taken outside of the conditional expectation. The third equality uses the Schur Gibbs property, see Definition \ref{DefSGP}. The first inequality on the third line holds if $N \geq N_4$ and uses Lemma \ref{LemmaAP1} with $\tilde{\epsilon} = \epsilon/2$  as well as the fact that on the event $E_N$ the random variables $\mathfrak{L}^N(-t_3), \mathfrak{L}^N(t_3)$ and $L^N_k \llbracket -t_3, t_3 \rrbracket$ (that play the roles of $\vec{x}, \vec{y}$ and $\ell_{bot}$) satisfy the inequalities 
	\begin{enumerate}
		\item $\sup_{s \in [- t_3,t_3]}\big[L^N_k(s)  - ps \big]  \leq M_2 (2t_3)^{1/2}$,
		\item  $-pt_3 + M_1 (2t_3)^{1/2} \geq  {L}^N_1(-t_3) \geq  {L}^N_{k-1}(-t_3) \geq \max\left(L^N_k(-t_3), -pt_3- M_1 (2t_3)^{1/2}\right),$
		\item $pt_3 + M_1 (2t_3)^{1/2} \geq {L}^N_1(t_3) \geq {L}^N_{k-1}(t_3) \geq  \max \left(L^N_k(t_3),  p t_3- M_1(2t_3)^{1/2} \right).$
	\end{enumerate}
	The last inequality in (\ref{boundoneEN}) is trivial.
	
	Combining (\ref{boundoneEN}) with (\ref{UBEC}), we see that for all $N \geq \max(N_2, N_4)$ we have
	$$\mathbb{P}\left( V  \right) = \mathbb{P}(V \cap E_N) + \mathbb{P}(V \cap E_N^c) \leq \epsilon/2 + \mathbb{P}(E_N^c) < \epsilon,$$
	which proves the proposition.
\end{proof}


%-------------------------------------------------------------------------------------------------------------------------------------------------------------------------------------------------
% Section 4.2
%
%-------------------------------------------------------------------------------------------------------------------------------------------------------------------------------------------------
\subsection{Proof of Theorem \ref{PropTightGood} }\label{Section4.2}

By Lemma \ref{2Tight}, it suffices to verify the following two conditions for all $i \in \llbracket 1,k-1\rrbracket$, $r>0$, and $\epsilon>0$:
\begin{equation}\label{ThmCond1}
\lim_{a\to\infty} \limsup_{N\to\infty} \pr(|f^N_i(0)|\geq a) = 0 
\end{equation}
\begin{equation}\label{ThmCond2}
\lim_{\delta\to 0} \limsup_{N\to\infty} \pr\left(\sup_{{x,y\in [-r,r], |x-y|\leq\delta}} |f^N_i(x) - f^N_i(y)| \geq \epsilon \right)= 0.
\end{equation}
For the sake of clarity, we will prove these conditions in several steps.\\

\noindent\textbf{Step 1.} In this step we prove \eqref{ThmCond1}. Let $\epsilon > 0$ be given. Then by Lemmas \ref{PropSup} and \ref{PropSup2} we can find $N_2, N_3$ and $R_1, R_2$ such that for $N \geq \max(N_1, N_2)$
\begin{align*}
\pr\left(\sup_{s\in[-t_3,t_3]} [L_1^N(s)-ps]\geq R_1N^{\alpha/2}\right)<\epsilon/2,\\
\pr\left(\inf_{s\in[-t_3,t_3]}[L_{k-1}^N(s)-ps]\leq -R_2 N^{\alpha/2}\right)<\epsilon/2.
\end{align*}
In particular, if we set $R  = \max(R_1, R_2)$ and utilize the fact that $L_1^N(0) \geq \cdots \geq L_{k-1}^N(0)$ we conclude that for any $i \in \llbracket 1, k-1 \rrbracket$ we have
$$\pr\big(|L_i^N(0)|\geq R N^{\alpha/2}\big)\leq \pr\big(L_1^N(0)\geq R_1 N^{\alpha/2}\big) + \pr\big(L_{k-1}^N(0)\leq -R_2N^{\alpha/2}\big) < \epsilon,$$
which implies \eqref{ThmCond1}.\\

\noindent\textbf{Step 2.} In this step we prove (\ref{ThmCond2}). In the sequel we fix $r, \epsilon > 0$ and $i \in \llbracket 1, k-1 \rrbracket$. To prove (\ref{ThmCond2}) it suffices to show that for any $\eta>0$, there exists a $\delta > 0$ and $N_0$ such that $N \geq N_0$ implies 
\begin{equation}\label{S2R1}
\pr\left(\sup_{{x,y\in [-r,r], |x-y|\leq\delta}} |f^N_i(x) - f^N_i(y)| \geq \epsilon\right)<\eta.
\end{equation}

For $\delta > 0$ we define the event
\begin{equation}\label{Adelta}
A^N_\delta =\left\{\sup_{{x,y\in [-t_1,t_1], |x-y|\leq \delta N^\alpha}} \abs*{L_i^N(x)-L_i^N(y)-p(x-y)}\geq \frac{3N^{\alpha/2}\epsilon}4\right\},
\end{equation}
where we recall that $t_1 = \lfloor (r + 1)N^{\alpha} \rfloor$ from (\ref{eqsts}). We claim that there exist $\delta_0 > 0$ and $N_0 \in \mathbb{N}$ such that for $\delta \in (0, \delta_0]$ and $N \geq N_0$ we have
\begin{equation}\label{Abound}
\mathbb{P}(A^N_\delta) < \eta.
\end{equation}
We prove (\ref{Abound}) in the steps below. Here we assume its validity and conclude the proof of (\ref{S2R1}).\\

Observe that if $\delta \in \left (0, \min \left(\delta_0, \epsilon \cdot (8 \lambda r)^{-1} \right) \right)$, where $\lambda$ is as in the statement of the theorem, we have the following tower of inequalities
\begin{equation}\label{Term1}
\begin{split}
&\pr\left(\sup_{{x,y\in [-r,r], |x-y|\leq\delta}} |f^N_i(x) - f^N_i(y)| \geq \epsilon\right) = \\
&\pr\left(\sup_{{x,y\in [-r,r],|x-y|\leq\delta}} \abs*{N^{-\alpha/2}\left(L^N_i(xN^{\alpha}) - L^N_i(yN^\alpha)\right)-p(x-y)N^{\alpha/2}+\lambda(x^2-y^2)} \geq \epsilon\right) \leq \\
&\pr\left(\sup_{{x,y\in [-r,r], |x-y|\leq\delta}} N^{-\alpha/2}\abs*{L_i^N(xN^\alpha)-L_i^N(yN^\alpha)-p(x-y)N^\alpha}+2\lambda r\delta\geq \epsilon\right) \leq \\
& \pr\left(\sup_{{x,y\in [-r,r], |x-y|\leq\delta}} \abs*{L_i^N(xN^\alpha)-L_i^N(yN^\alpha)-p(x-y)N^\alpha}\geq \frac{3N^{\alpha/2}\epsilon}4\right)\leq \mathbb{P}(A^N_\delta) < \eta .
\end{split}
\end{equation}
In (\ref{Term1}) the first equality follows from the definition of $f_i^N$, and the inequality on the second line follows from the inequality $|x^2-y^2|\leq 2r\delta$, which holds for all $x,y \in [-r,r]$ such that $|x-y| \leq \delta$. The inequality in the third line of (\ref{Term1}) follows from our assumption that $\delta <   \epsilon \cdot (8 \lambda r)^{-1}$ and the first inequality on the last line follows from the definition of $A^N_\delta$ in (\ref{Adelta}), and the fact that $t_1 \geq r N^{\alpha}$. The last inequality follows from our assumption that $\delta < \delta_0$ and (\ref{Abound}). In view of (\ref{Term1}) we conclude (\ref{S2R1}).\\

{\bf \raggedleft Step 3.} In this step we prove (\ref{Abound}) and fix $\eta > 0$ in the sequel. For $\delta_1, M_1 > 0$ and $N \in \mathbb{N}$ we define the events
\begin{equation}
\begin{split}
E_1= \hspace{-0.5mm}\left\{\max_{1\leq j \leq k-1}\abs*{L_j^N(\pm t_1) \mp pt_1}\leq M_1N^{\alpha/2} \right\}, E_2=\hspace{-0.5mm}\left\{Z(-t_1, t_1, \vec x, \vec y, \infty, L_{k}^N\llbracket -t_1, t_1 \rrbracket)>\delta_1\right\},
\end{split}
\end{equation}
where we used the same notation as in Proposition \ref{PropMain} (in particular $\vec x = (L^N_1(-t_1), \dots, L_{k-1}^N(-t_1))$ and $\vec y = (L_1^N(t_1), \dots, L_{k-1}^N(t_1))$). Combining Lemmas \ref{PropSup}, \ref{PropSup2} and Proposition \ref{PropMain} we know that we can find $\delta_1 > 0$ sufficiently small, $M_1$ sufficiently large and $\tilde{N} \in \mathbb{N}$ such that for $N \geq \tilde{N}$ we know
\begin{equation}\label{BoundECup}
\mathbb{P} \left(E_1^c \cup E_2^c \right) < \eta/2.
\end{equation}
We claim that we can find $\delta_0 > 0$ and $N_0 \geq \tilde{N}$ such that for $N \geq N_0$ and $\delta \in (0, \delta_0)$ we have
\begin{equation}\label{Abound2}
\mathbb{P}(A^N_\delta \cap E_1 \cap E_2 ) < \eta/2.
\end{equation}
Since
$$\pr(A^N_\delta)= \pr(A^N_\delta\cap E_1\cap E_2)+\pr(A^N_\delta\cap\left(E_1^c\cup E_2^c\right))\leq \pr(A^N_\delta\cap E_1\cap E_2)+\mathbb{P} \left(E_1^c \cup E_2^c \right),$$
we see that (\ref{BoundECup}) and (\ref{Abound2}) together imply (\ref{Abound}).\\

{\bf \raggedleft Step 4.} In this step we prove (\ref{Abound2}). We define the $\sigma$-algebra 
$$\mathcal{F}=\sigma\left(L_{k}^N \llbracket -t_1, t_1 \rrbracket ,L_1^N(\pm t_1 ), L_2^N(\pm t_1 ),\dots, L_{k-1}^N(\pm t_1 )\right).$$
Clearly $E_1, E_2\in \mathcal{F}$, so the indicator random variables $\indic_{E_1}$ and $\indic_{E_2}$ are $\mathcal{F}$-measurable. It follows from the tower property of conditional expectation that
\begin{equation}\label{tower}
\pr\left(A^N_\delta\cap E_1\cap E_2\right)=\ex\left[\indic_{A^N_\delta} \indic_{E_1} \indic_{E_2}\right] =\ex\left[\indic_{E_1} \indic_{E_2}\ex\left[\indic_{A^N_\delta}\mid \mathcal{F}\right]\right]. 
\end{equation}
By the Schur-Gibbs property (see Definition \ref{DefSGP}), we know that $\mathbb{P}$-almost surely
\begin{equation}\label{tower2}
\ex\left[\indic_{A^N_\delta}\mid \mathcal{F}\right]=\ex_{avoid,Ber}^{-t_1,t_1,\vec x, \vec y, \infty, L_{k}^N \llbracket -t_1, t_1 \rrbracket}\left[\indic_{A^N_\delta}\right].
\end{equation}
We now observe that the Radon-Nikodym derivative of $\pr_{avoid,Ber}^{-t_1,t_1,\vec x, \vec y, \infty, L_{k}^N \llbracket -t_1, t_1 \rrbracket}$ with respect to $\pr_{Ber}^{-t_1, t_1,\vec x,\vec y}$ is given by 
\begin{equation}\label{RN}
\frac{d\pr_{avoid,Ber}^{-t_1,t_1,\vec x, \vec y, \infty, L_{k}^N\llbracket -t_1, t_1 \rrbracket } (Q_1, \dots, Q_{k-1})}{d\pr_{Ber}^{-t_1, t_1,\vec x,\vec y}} = \frac{\indic_{\left\{Q_1 \geq \cdots \geq Q_{k-1} \geq Q_k \right\}}}{Z(-t_1,t_1,\vec x, \vec y, \infty,  L_{k}^N\llbracket -t_1, t_1 \rrbracket )},
\end{equation}
where $\mathfrak{Q} = (Q_1, \dots, Q_{k-1})$ is $\pr_{Ber}^{-t_1, t_1,\vec x,\vec y}$-distributed and $Q_k = L_{k}^N\llbracket -t_1, t_1 \rrbracket$. To see this, note that by Definition \ref{DefAvoidingLawBer} we have for any set $A \subset  \prod_{i = 1}^{k-1}\Omega(-t_1, t_1, x_i, y_i )$ that 
\begin{equation*}
\begin{split}
&\pr_{avoid,Ber}^{-t_1,t_1,\vec x, \vec y, \infty, L_{k}^N\llbracket -t_1, t_1 \rrbracket}(A) = \frac{\pr_{Ber}^{-t_1,t_1,\vec x, \vec y}(A\cap\left\{Q_1 \geq \cdots \geq Q_{k-1} \geq Q_k\right\})}{\pr_{Ber}^{-t_1,t_1,\vec x, \vec y}(Q_1\geq\cdots\geq Q_{k-1} \geq Q_k)} = \\
& \frac{\ex_{Ber}^{-t_1,t_1,\vec x, \vec y}\left[\indic_A \cdot  \indic_{\left\{Q_1\geq\cdots\geq Q_{k-1} \geq Q_k \right\}}\right]}{Z(-t_1,t_1,\vec{x},\vec{y}, \infty, L^N_{k} \llbracket -t_1, t_1 \rrbracket)} = \int_A \frac{\indic_{\left\{Q_1\geq\cdots\geq Q_{k-1} \geq Q_k \right\}}}{Z(-t_1,t_1,\vec x, \vec y, \infty, L_{k}^N \llbracket -t_1, t_1 \rrbracket )}\,d\pr_{Ber}^{-t_1,t_1,\vec x, \vec y}.
\end{split}
\end{equation*}
It follows from \eqref{tower}, \eqref{RN}, and the definition of $E_2$ that
\begin{equation}\label{RT1}
\begin{split}
&\pr(A^N_\delta\cap E_1\cap E_2) =\ex\left[\indic_{E_1}\indic_{E_2} \ex_{Ber}^{-t_1, t_1,\vec x,\vec y}\left[\frac{\indic_{B^N_\delta}\cdot \indic_{\left\{Q_1\geq\cdots\geq Q_{k}\right\}}}{Z(-t_1,t_1,\vec x, \vec y, L^N_{k} \llbracket -t_1, t_1 \rrbracket)}\right]\right] \leq \\
&\leq \ex\left[\indic_{E_1}\indic_{E_2}\ex_{Ber}^{-t_1,t_1,\vec x,\vec y}\left[\frac{\indic_{B^N_\delta}}{\delta_1}\right]\right] \leq \frac{1}{\delta_1} \ex\left[ \indic_{E_1} \cdot\pr_{Ber}^{-t_1,t_1,\vec{x}, \vec{y} }(B^N_\delta) \right],
\end{split}
\end{equation}
where 
$$B^N_\delta = \left\{\sup_{{x,y\in [-t_1,t_1], |x-y|\leq \delta N^\alpha}} \abs*{Q_i(x)-Q_i(y)-p(x-y)}\geq \frac{3N^{\alpha/2}\epsilon}4\right\}.$$
Notice that under $\pr_{Ber}^{-t_1,t_1,\vec{x}, \vec{y} }$ the law of $Q_i$ is precisely $\pr_{Ber}^{-t_1,t_1,x_i, y_i }$, and so we conclude that 
\begin{equation}\label{RT2}
\begin{split}
& \pr_{Ber}^{-t_1,t_1,\vec{x}, \vec{y} }(B^N_\delta) = \pr_{Ber}^{0,2t_1,0, y_i - x_i }\left( \sup_{{x,y\in [0,2t_1], |x-y|\leq \delta N^\alpha}} \abs*{\ell(x)-\ell(y)-p(x-y)}\geq \frac{3N^{\alpha/2}\epsilon}4  \right),
\end{split}
\end{equation}
where $\ell$ has law $\pr_{Ber}^{0,2t_1,0, y_i - x_i }$ (note that in (\ref{RT2}) we implicitly translated the path $\ell$ to the right by $t_1$ and up by $-x_i$, which does not affect the probability in question). Since on the event $E_1$ we know that $|y_i -x_i - 2 p t_1| \leq 2M_1 N^{\alpha}$  we conclude from Lemma \ref{MOCLemmaS4} that we can find $N_0$ and $\delta_0 > 0$ depending on $M_1, r, \alpha$ such that for $N \geq N_0$ and $\delta \in (0, \delta_0)$ we have
\begin{equation}\label{RT3}
\begin{split}
& \indic_{E_1} \cdot \pr_{Ber}^{0,2t_1,0, y_i - x_i }\left( \sup_{{x,y\in [0,2t_1], |x-y|\leq \delta N^\alpha}} \abs*{\ell(x)-\ell(y)-p(x-y)}\geq \frac{3N^{\alpha/2}\epsilon}4  \right) < \frac{\delta_1 \eta}{2}.
\end{split}
\end{equation}
Combining (\ref{RT1}), (\ref{RT2}) and (\ref{RT3}) we conclude (\ref{Abound2}), and hence the theorem.

